documentation (fragments) for expressiveness prices and bisimilarity; direct_expr definition in formula_prices_list

formula_prices_list.thy
@@ -1,9 +1,37 @@
+(*<*)
 theory formula_prices_list
   imports 
     Main
     HML_list
     "HOL-Library.Extended_Nat"
 begin
+(*>*)
+
+section \<open>Price Spectra of Behavioral Equivalences\<close>
+
+text \<open>The linear-time--branching-time spectrum can be represented in terms of HML-expressiveness (s.h. section HML).
+(Deciding all at once)(energy games) show how one can think of the amount of HML-expressiveness used by a formula by its \textit{price}.
+The equivalences of the spectrum (or their modal-logical characterizations) can then be defined in terms of \textit{price coordinates}, that is
+equivalence $X$ is characterized by the HML formulas with prices less then or equal to a \textit{X-price bound} $e_X$.
+We use the six dimensions from (energy games) to characterize the notions of equivalence we are interested in (In figure xx oder so umschreiben).
+Intuitively, the dimensions can be described as follows:\\
+1. Observations\\
+...
+...\\ \<close>
+
+subsubsection \<open>Formula Prices\<close>
+text \<open>The \textit{expressiveness price} $\text{expr}: \text{HML}[\Sigma] \rightarrow (\mathbb{N} \cup \{\infty\})^6$ of a formula is defined recursively, similar to energy games:
+TODO: $\text{expr}$ function \\\\
+
+Remark: Infinity is included in our definition, due to infinite branching conjunctions. Supremum over infinite set wird zu unendlich.\<close>
+
+text \<open>To better argue about the function we define each dimension as a seperate function.\<close>
+
+text \<open>Vlt als erstes: modaltiefe als beispiel für observation expressiveness von formel, mit isabelle definition,
+dann pos\_r definition,
+direct\_expr definition,
+einzelne dimensionen,
+lemma direct\_expr = expr...\<close>
 
 primrec expr_1 :: "('a, 's)hml \<Rightarrow> enat"
   where
@@ -12,6 +40,65 @@ expr_1_conj: \<open>expr_1 (hml_conj I J \<Phi>) = Sup ((expr_1 \<circ> \<Phi>) 
 expr_1_pos: \<open>expr_1 (hml_pos \<alpha> \<phi>) = 
   1 + (expr_1 \<phi>)\<close>
 
+fun pos_r :: "('a, 's)hml set \<Rightarrow> ('a, 's)hml set"
+  where
+"pos_r xs = (
+let max_val = (Sup (expr_1 ` xs)); 
+  max_elem = (SOME \<psi>. \<psi> \<in> xs \<and> expr_1 \<psi> = max_val);
+  xs_new = xs - {max_elem}
+in xs_new)"
+
+lemma pos_r_subs: "pos_r (\<Phi> ` I) \<subseteq> (\<Phi> ` I)"
+  by auto
+
+function direct_expr :: "('a, 's)hml \<Rightarrow> enat \<times> enat \<times> enat \<times> enat \<times> enat \<times> enat" where
+  "direct_expr TT = (0, 1, 0, 0, 0, 0)" |
+  "direct_expr (hml_pos \<alpha> \<phi>) = (1 + fst (direct_expr \<phi>), 
+                                fst (snd (direct_expr \<phi>)), 
+                                fst (snd (snd (direct_expr \<phi>))), 
+                                fst (snd (snd (snd (direct_expr \<phi>)))), 
+                                fst (snd (snd (snd (snd (direct_expr \<phi>))))), 
+                                snd (snd (snd (snd (snd (direct_expr \<phi>))))))" |
+  "direct_expr (hml_conj I J \<Phi>) = (Sup ((fst \<circ> direct_expr \<circ> \<Phi>) ` I \<union> (fst \<circ> direct_expr \<circ> \<Phi>) ` J), 
+                                    1 + Sup ((fst \<circ> snd \<circ> direct_expr \<circ> \<Phi>) ` I \<union> (fst \<circ> snd \<circ> direct_expr \<circ> \<Phi>) ` J), 
+(Sup ((fst \<circ> direct_expr \<circ> \<Phi>) ` I \<union> (fst \<circ> snd \<circ> snd \<circ> direct_expr \<circ> \<Phi>) ` I \<union> (fst \<circ> snd \<circ> snd \<circ> direct_expr \<circ> \<Phi>) ` J)),
+(Sup (((fst \<circ> direct_expr) ` (pos_r (\<Phi> ` I)))  \<union> (fst \<circ> snd \<circ> snd \<circ> snd \<circ> direct_expr \<circ> \<Phi>) ` I \<union> (fst \<circ> snd \<circ> snd \<circ> snd \<circ> direct_expr \<circ> \<Phi>) ` J)),  
+(Sup ((fst \<circ> snd \<circ> snd \<circ> snd \<circ> snd \<circ> direct_expr \<circ> \<Phi>) ` I \<union> (fst \<circ> snd \<circ> snd \<circ> snd \<circ> snd \<circ> direct_expr \<circ> \<Phi>) ` J \<union> (fst \<circ> direct_expr \<circ> \<Phi>) ` J)), 
+(Sup ((snd \<circ> snd \<circ> snd \<circ> snd \<circ> snd \<circ> direct_expr \<circ> \<Phi>) ` I \<union> ((eSuc \<circ> snd \<circ> snd \<circ> snd \<circ> snd \<circ> snd \<circ> direct_expr \<circ> \<Phi>) ` J))))"
+  by ((meson hml.exhaust), simp+)
+
+inductive_set HML_wf_rel :: "(('a, 's)hml) rel" where
+"\<phi> = \<Phi> i \<and> i \<in> (I \<union> J) \<Longrightarrow> (\<phi>, (hml_conj I J \<Phi>)) \<in> HML_wf_rel" |
+"(\<phi>, (hml_pos \<alpha> \<phi>)) \<in> HML_wf_rel"
+
+lemma HML_wf_rel_is_wf: \<open>wf HML_wf_rel\<close>
+  unfolding wf_def
+proof safe
+  fix P
+  assume assm: "\<forall>x. (\<forall>y. (y, x) \<in> HML_wf_rel \<longrightarrow> P y) \<longrightarrow> P x"
+  show "\<And>\<phi>. P \<phi>" proof-
+    fix \<phi>
+    show "P \<phi>" proof(induction \<phi>)
+    case TT
+    then show ?case 
+      using HML_wf_rel.cases assm by blast
+  next
+    case (hml_pos x1 \<phi>)
+    then show ?case 
+      using HML_wf_rel.cases hml.inject hml.simps assm 
+      by (smt (verit, best))
+  next
+    case (hml_conj x1 x2 x3)
+    then show ?case 
+      using assm
+      by (metis HML_wf_rel.cases hml.inject(2) hml.simps(8) rangeI)
+    qed
+  qed
+qed
+
+termination
+  apply rule
+  using HML_wf_rel_is_wf HML_wf_rel.simps Un_iff pos_r_subs by fastforce+
 
 primrec expr_2 :: "('a, 's)hml \<Rightarrow> enat"
   where
@@ -25,14 +112,6 @@ primrec expr_3 :: "('a, 's) hml \<Rightarrow> enat"
 expr_3_tt: \<open>expr_3 TT = 0\<close> |
  expr_3_pos: \<open>expr_3 (hml_pos \<alpha> \<phi>) = expr_3 \<phi>\<close> | 
 expr_3_conj: \<open>expr_3 (hml_conj I J \<Phi>) = (Sup ((expr_1 \<circ> \<Phi>) ` I \<union> (expr_3 \<circ> \<Phi>) ` I \<union> (expr_3 \<circ> \<Phi>) ` J))\<close>
-
-fun pos_r :: "('a, 's)hml set \<Rightarrow> ('a, 's)hml set"
-  where
-"pos_r xs = (
-let max_val = (Sup (expr_1 ` xs)); 
-max_elem = (SOME \<psi>. \<psi> \<in> xs \<and> expr_1 \<psi> = max_val);
-xs_new = xs - {max_elem}
-in xs_new)"
 
 primrec expr_4 :: "('a, 's)hml \<Rightarrow> enat" 
   where
@@ -58,5 +137,169 @@ expr_6_conj: \<open>expr_6 (hml_conj I J \<Phi>) =
 fun expr :: "('a, 's)hml \<Rightarrow> enat \<times> enat \<times> enat \<times>  enat \<times> enat \<times> enat" 
   where
 \<open>expr \<phi> = (expr_1 \<phi>, expr_2 \<phi>, expr_3 \<phi>, expr_4 \<phi>, expr_5 \<phi>, expr_6 \<phi>)\<close>
-                                 
+
+lemma apply_comp:
+  assumes "\<forall>x \<in> \<Phi> ` I. F x = G1 (G2 (G3 (G4 (G5 ((H x))))))"
+  shows "Sup ((F \<circ> \<Phi>) ` I) = Sup((G1 \<circ> G2 \<circ> G3 \<circ> G4 \<circ> G5 \<circ> H \<circ> \<Phi>) ` I)"
+  using assms by auto
+
+lemma fa_set_eq: 
+  assumes "\<forall>x \<in> \<Phi> ` I. F x = G (H x)"
+  shows "((F \<circ> \<Phi>) ` I) = (G \<circ> H \<circ> \<Phi>) ` I" 
+  using assms by force
+
+lemma expr_6_direct_expr_eq:
+  assumes "\<And>x. x \<in> \<Phi> ` I \<Longrightarrow> expr_6 x = snd (snd (snd (snd (snd (direct_expr x)))))"
+  shows "(expr_6 \<circ> \<Phi>) ` I = (snd \<circ> snd \<circ> snd \<circ> snd \<circ> snd \<circ> direct_expr \<circ> \<Phi>) ` I"
+proof -
+  have "(expr_6 \<circ> \<Phi>) ` I = (\<lambda>x. snd (snd (snd (snd (snd (direct_expr (\<Phi> x))))))) ` I"
+    by (simp add: assms)
+  also have "... = (snd \<circ> snd \<circ> snd \<circ> snd \<circ> snd \<circ> direct_expr \<circ> \<Phi>) ` I"
+    by auto
+  finally show ?thesis .
+qed
+
+lemma expr_6_eSuc_eq:
+  assumes "\<And>x. x \<in> \<Phi> ` J \<Longrightarrow> eSuc (expr_6 x) = eSuc (snd (snd (snd (snd (snd (direct_expr x))))))"
+  shows "((eSuc \<circ> expr_6 \<circ> \<Phi>) ` J) = ((eSuc \<circ> snd \<circ> snd \<circ> snd \<circ> snd \<circ> snd \<circ> direct_expr \<circ> \<Phi>) ` J)"
+proof-
+  have "((eSuc \<circ> expr_6 \<circ> \<Phi>) ` J) = (\<lambda>x. eSuc (snd (snd (snd (snd (snd (direct_expr (\<Phi> x)))))))) ` J"
+    using assms by force
+  also have "... = ((eSuc \<circ> snd \<circ> snd \<circ> snd \<circ> snd \<circ> snd \<circ> direct_expr \<circ> \<Phi>) ` J)"
+    by auto
+  finally show ?thesis.
+qed
+
+lemma expr_5_dir_eq:
+  assumes "\<forall>x \<in> \<Phi> ` (I \<union> J). expr_5 x = fst (snd (snd (snd (snd (direct_expr x)))))"
+  shows "((expr_5 \<circ> \<Phi>) ` I \<union> (expr_5 \<circ> \<Phi>) ` J) = 
+          ((fst \<circ> snd \<circ> snd \<circ> snd \<circ> snd \<circ> direct_expr \<circ> \<Phi>) ` I \<union> (fst \<circ> snd \<circ> snd \<circ> snd \<circ> snd \<circ> direct_expr \<circ> \<Phi>) ` J)"
+proof-
+  have "((expr_5 \<circ> \<Phi>) ` I \<union> (expr_5 \<circ> \<Phi>) ` J) = (\<lambda>x. fst (snd (snd (snd (snd (direct_expr (\<Phi> x))))))) ` (I \<union> J)"
+    using assms 
+    by auto
+  also have "... = (fst \<circ> snd \<circ> snd \<circ> snd \<circ> snd \<circ> direct_expr \<circ> \<Phi>) ` (I \<union> J)"
+    by auto 
+  also have "... =  ((fst \<circ> snd \<circ> snd \<circ> snd \<circ> snd \<circ> direct_expr \<circ> \<Phi>) ` I \<union> (fst \<circ> snd \<circ> snd \<circ> snd \<circ> snd \<circ> direct_expr \<circ> \<Phi>) ` J)"
+    by blast
+  finally show ?thesis.
+qed
+
+thm comp_apply
+
+lemma 
+  shows "expr \<phi> = direct_expr \<phi>"
+proof(induction \<phi>)
+  case TT
+  have "expr TT = (0, 1, 0, 0, 0, 0)" using expr.simps expr_1.simps(1) expr_2.simps(1) expr_3.simps(1) expr_4.simps(1) expr_5.simps(1) expr_6.simps(1)
+    by force
+  then show ?case using direct_expr.simps(1) 
+    by force
+next
+  case (hml_pos \<alpha> \<phi>)
+  hence IH: "(expr_1 \<phi>, expr_2 \<phi>, expr_3 \<phi>, expr_4 \<phi>, expr_5 \<phi>, expr_6 \<phi>) =
+                                (fst (direct_expr \<phi>), 
+                                fst (snd (direct_expr \<phi>)), 
+                                fst (snd (snd (direct_expr \<phi>))), 
+                                fst (snd (snd (snd (direct_expr \<phi>)))), 
+                                fst (snd (snd (snd (snd (direct_expr \<phi>))))), 
+                                snd (snd (snd (snd (snd (direct_expr \<phi>))))))"
+    by auto
+  have expr: "expr (hml_pos \<alpha> \<phi>) = (1 + (expr_1 \<phi>), expr_2 \<phi>, expr_3 \<phi>, expr_4 \<phi>, expr_5 \<phi>, expr_6 \<phi>)"
+    using expr.simps expr_1.simps expr_2.simps expr_3.simps expr_4.simps expr_5.simps expr_6.simps
+    by simp
+  have "direct_expr (hml_pos \<alpha> \<phi>) = 
+                                (1 + fst (direct_expr \<phi>), 
+                                fst (snd (direct_expr \<phi>)), 
+                                fst (snd (snd (direct_expr \<phi>))), 
+                                fst (snd (snd (snd (direct_expr \<phi>)))), 
+                                fst (snd (snd (snd (snd (direct_expr \<phi>))))), 
+                                snd (snd (snd (snd (snd (direct_expr \<phi>))))))"
+    using direct_expr.simps(2) by auto
+  then show ?case using expr IH by force
+next
+  case (hml_conj I J \<Phi>)
+  hence IH: "\<forall>\<phi> \<in> \<Phi> ` I. (expr_1 \<phi>, expr_2 \<phi>, expr_3 \<phi>, expr_4 \<phi>, expr_5 \<phi>, expr_6 \<phi>) =
+                                (fst (direct_expr \<phi>), 
+                                fst (snd (direct_expr \<phi>)), 
+                                fst (snd (snd (direct_expr \<phi>))), 
+                                fst (snd (snd (snd (direct_expr \<phi>)))), 
+                                fst (snd (snd (snd (snd (direct_expr \<phi>))))), 
+                                snd (snd (snd (snd (snd (direct_expr \<phi>))))))"
+        "\<forall>\<phi> \<in> \<Phi> ` J. (expr_1 \<phi>, expr_2 \<phi>, expr_3 \<phi>, expr_4 \<phi>, expr_5 \<phi>, expr_6 \<phi>) =
+                                (fst (direct_expr \<phi>), 
+                                fst (snd (direct_expr \<phi>)), 
+                                fst (snd (snd (direct_expr \<phi>))), 
+                                fst (snd (snd (snd (direct_expr \<phi>)))), 
+                                fst (snd (snd (snd (snd (direct_expr \<phi>))))), 
+                                snd (snd (snd (snd (snd (direct_expr \<phi>))))))"
+    by simp+
+  hence e1: "Sup ((expr_1 \<circ> \<Phi>) ` I \<union> (expr_1 \<circ> \<Phi>) ` J) = Sup ((fst \<circ> direct_expr \<circ> \<Phi>) ` I \<union> (fst \<circ> direct_expr \<circ> \<Phi>) ` J)"
+    by (smt (verit, best) Pair_inject comp_apply image_cong image_eqI)
+  have e2: "1 + Sup ((expr_2 \<circ> \<Phi>) ` I \<union> (expr_2 \<circ> \<Phi>) ` J) = 1 + Sup ((fst \<circ> snd \<circ> direct_expr \<circ> \<Phi>) ` I \<union> (fst \<circ> snd \<circ> direct_expr \<circ> \<Phi>) ` J)"
+    using IH Sup_le_iff 
+    by (smt (verit) Pair_inject comp_apply image_cong image_eqI)
+  have e3: "(Sup ((expr_1 \<circ> \<Phi>) ` I \<union> (expr_3 \<circ> \<Phi>) ` I \<union> (expr_3 \<circ> \<Phi>) ` J)) =
+        (Sup ((fst \<circ> direct_expr \<circ> \<Phi>) ` I \<union> (fst \<circ> snd \<circ> snd \<circ> direct_expr \<circ> \<Phi>) ` I \<union> (fst \<circ> snd \<circ> snd \<circ> direct_expr \<circ> \<Phi>) ` J))"
+    using IH Sup_le_iff 
+    by (smt (verit, ccfv_SIG) Pair_inject comp_apply image_comp image_cong)
+  have e4: "Sup ((expr_1 ` (pos_r (\<Phi> ` I)))  \<union> (expr_4 \<circ> \<Phi>) ` I \<union> (expr_4 \<circ> \<Phi>) ` J) =
+        (Sup (((fst \<circ> direct_expr) ` (pos_r (\<Phi> ` I)))  \<union> (fst \<circ> snd \<circ> snd \<circ> snd \<circ> direct_expr \<circ> \<Phi>) ` I \<union> (fst \<circ> snd \<circ> snd \<circ> snd \<circ> direct_expr \<circ> \<Phi>) ` J))"
+  proof-
+    have sup_pos_r: "\<forall>x \<in> pos_r (\<Phi> ` I). expr_1 x = (fst \<circ> direct_expr) x"
+      using IH 
+      by (metis (no_types, lifting) Diff_iff Pair_inject comp_apply pos_r.simps)
+    hence "Sup (expr_1 ` pos_r (\<Phi> ` I)) = Sup ((fst \<circ> direct_expr) ` pos_r (\<Phi> ` I))"
+      by (meson SUP_cong)
+    have "\<forall>x \<in> \<Phi> ` (I \<union> J). expr_4 x = fst (snd (snd (snd (direct_expr x))))"
+      using IH
+      by blast+
+    hence "Sup ((expr_4 \<circ> \<Phi>) ` I \<union> (expr_4 \<circ> \<Phi>) ` J) = 
+          Sup ((fst \<circ> snd \<circ> snd \<circ> snd \<circ> direct_expr \<circ> \<Phi>) ` I \<union>
+          (fst \<circ> snd \<circ> snd \<circ> snd \<circ> direct_expr \<circ> \<Phi>) ` J)"
+      using SUP_cong by auto
+    then show ?thesis using sup_pos_r 
+      by (metis (no_types, lifting) Sup_union_distrib image_cong inf_sup_aci(6))
+  qed
+  have e5: "(Sup ((expr_5 \<circ> \<Phi>) ` I \<union> (expr_5 \<circ> \<Phi>) ` J \<union> (expr_1 \<circ> \<Phi>) ` J)) =
+  (Sup ((fst \<circ> snd \<circ> snd \<circ> snd \<circ> snd \<circ> direct_expr \<circ> \<Phi>) ` I \<union> (fst \<circ> snd \<circ> snd \<circ> snd \<circ> snd \<circ> direct_expr \<circ> \<Phi>) ` J \<union> (fst \<circ> direct_expr \<circ> \<Phi>) ` J))"
+    using IH
+  proof-
+    have fa_e5: "\<forall>x \<in> \<Phi> ` (I \<union> J). expr_5 x = fst (snd (snd (snd (snd (direct_expr x)))))"
+          "\<forall>x \<in> \<Phi> ` J. expr_1 x = fst (direct_expr x)"
+      using IH 
+      by blast+
+    hence "Sup ((expr_1 \<circ> \<Phi>) ` J )= Sup ((fst \<circ> direct_expr \<circ> \<Phi>) ` J)" 
+      by fastforce
+    have "Sup ((expr_5 \<circ> \<Phi>) ` I \<union> (expr_5 \<circ> \<Phi>) ` J) = 
+          Sup ((fst \<circ> snd \<circ> snd \<circ> snd \<circ> snd \<circ> direct_expr \<circ> \<Phi>) ` I \<union> (fst \<circ> snd \<circ> snd \<circ> snd \<circ> snd \<circ> direct_expr \<circ> \<Phi>) ` J)"
+      using expr_5_dir_eq fa_e5 by force
+    then show ?thesis 
+      using \<open>Sup ((expr_1 \<circ> \<Phi>) ` J )= Sup ((fst \<circ> direct_expr \<circ> \<Phi>) ` J)\<close> 
+      by (simp add: Sup_union_distrib)
+  qed
+
+  have e6: "(Sup ((expr_6 \<circ> \<Phi>) ` I \<union> ((eSuc \<circ> expr_6 \<circ> \<Phi>) ` J))) =
+        (Sup ((snd \<circ> snd \<circ> snd \<circ> snd \<circ> snd \<circ> direct_expr \<circ> \<Phi>) ` I \<union> ((eSuc \<circ> snd \<circ> snd \<circ> snd \<circ> snd \<circ> snd \<circ> direct_expr \<circ> \<Phi>) ` J)))"
+  proof-
+    have "\<forall>x \<in> \<Phi> ` I. expr_6 x = snd (snd (snd (snd (snd (direct_expr x)))))"
+          "\<forall>x \<in> \<Phi> ` J. expr_6 x = snd (snd (snd (snd (snd (direct_expr x)))))"
+      using IH by blast+
+    from this(1) have "((expr_6 \<circ> \<Phi>) ` I) = ((snd \<circ> snd \<circ> snd \<circ> snd \<circ> snd \<circ> direct_expr \<circ> \<Phi>) ` I)"
+      using expr_6_direct_expr_eq by force
+    hence "Sup ((expr_6 \<circ> \<Phi>) ` I) = Sup ((snd \<circ> snd \<circ> snd \<circ> snd \<circ> snd \<circ> direct_expr \<circ> \<Phi>) ` I)"
+      by presburger 
+    have "\<forall>x \<in> \<Phi> ` J. eSuc (expr_6 x) = eSuc (snd (snd (snd (snd (snd (direct_expr x))))))"
+      using \<open>\<forall>x \<in> \<Phi> ` J. expr_6 x = snd (snd (snd (snd (snd (direct_expr x)))))\<close> by simp
+    hence "Sup ((eSuc \<circ> expr_6 \<circ> \<Phi>) ` J) = Sup ((eSuc \<circ> snd \<circ> snd \<circ> snd \<circ> snd \<circ> snd \<circ> direct_expr \<circ> \<Phi>) ` J)"
+      using expr_6_eSuc_eq by auto
+    then show ?thesis using \<open>Sup ((expr_6 \<circ> \<Phi>) ` I) = Sup ((snd \<circ> snd \<circ> snd \<circ> snd \<circ> snd \<circ> direct_expr \<circ> \<Phi>) ` I)\<close>
+      by (simp add: Sup_union_distrib)
+  qed
+
+  then show ?case using e1 e2 e3 e4 e5 e6 by simp
+qed
+
+(*<*)
 end
+(*>*)
