Equivalences.thy
@@ -1,0 +1,33 @@
+(*<*)
+theory Equivalences
+imports Transition_Systems
+begin
+(*>*)
+
+section \<open>Behavioral Equivalence of Processes\<close>
+
+text \<open>As discussed in the previous sections, LTSs model the behaviour of reactive systems. That behaviour
+is observable by the environment in terms of transitions performed by the system. Depending on different criteria
+on what constitutes equal behavior has led to a large number of equivalences for concurrent processes. Those equivalences are often
+defined in term of relations on LTSs or sets of executions. The finest commonly used \textit{extensional behavioral equivalence}
+is \textit{Bisimilarity}. In extensional equivalences, only observable behavior is taken into account, without considering the
+identity of the processes. This sets bisimilarity apart from stronger graph equivalences like \textit{graph isomorphism}, 
+here the (intensional) identity of processes is relevant. The coarsest commonly used equivalence is \textit{trace equivalence}.
+
+- LT-BT spectrum (between them there is a lattice of equivalences ...)
+- Wir behandeln bisimilarität hier gesondert wegen dessen bezihung zu HML (HM-Theorem) (s.h. Introduction, doppelung vermeiden).
+- example bisimilarity
+
+Informally, we call two processes bisimilar if...\<close>
+
+
+subsubsection \<open>Bisimilarity\<close>
+text \<open>The notion of strong bisimilarity can be formalised through \emph{strong bisimulation} (SB) relations, introduced originally in (citation Park). 
+A binary relation $\mathcal{R}$ over the set of processes $\Proc$ is an SB iff for all $(p,q) \in \mathcal{R}$:
+\begin{align*}
+&\forall p' \in \Proc,\; \alpha \in \Act .\; p \xrightarrow{\alpha} p' \longrightarrow
+\exists q' \in \Proc .\; q \xrightarrow{\alpha} q' \wedge (p',q') \in \mathcal{R}, \text{ and}\\
+&\forall q' \in \Proc,\; \alpha \in \Act .\; q \xrightarrow{\alpha} q' \longrightarrow
+\exists p' \in \Proc .\; p \xrightarrow{\alpha} p' \wedge (p',q') \in \mathcal{R}.
+\end{align*}\<close>
+end
