HML.thy
@@ -1,0 +1,147 @@
+(*<*)
+theory HML
+imports Main Transition_Systems
+begin
+(*>*)
+
+section \<open>Hennessy--Milner logic\<close>
+text \<open>For the purpose of this thesis, we focus on the modal-logical characterizations of equivalences, using Hennessy--Milner logic (HML). 
+First introduced by Matthew Hennessy and Robin Milner (citation), HML is a modal logic for expressing properties of systems described by LTS.
+Intuitively, HML describes observations on an LTS and two processes are considered equivalent under HML when there exists no observation that distinguishes between them.
+(citation) defined the modal-logical language as consisting of (finite) conjunctions, negations and a (modal) possibility operator:
+$$\varphi ::= t\!t \mid \varphi_1 \;\wedge\; \varphi_2 \mid \neg\varphi \mid \langle\alpha\rangle\varphi$$
+(where $\alpha$ ranges over the set of actions. The paper also proves that this characterization of strong bisimilarity
+corresponds to a relational definition that is effectively the same as in (...). Their result can be expressed as follows:
+for image-finite LTSs, two processes are strongly bisimilar iff they satisfy the same set of HML formulas. We call this the modal characterisation of
+strong bisimilarity. By allowing for conjunction of arbitrary width (infinitary HML), the modal characterization of strong bisimilarity can be proved for arbitrary LTS. This is done in (...)\<close>
+
+
+text \<open>Mention: HML to capture equivalences (Spectrum, HM theorem)\<close>
+subsubsection \<open>Hennessy--Milner logic\<close>
+text \<open>The syntax of Hennessy--Milner logic over a set $\Sigma$ of actions, (HML) - richtige font!!!!![$\Sigma$], is defined by the grammar:
+\begin{align*}
+    \varphi &::= \langle a \rangle \varphi && \text{with } a \in \Sigma \\
+            &\quad | \, \bigwedge_{i \in I} \psi_i \\
+    \psi &::= \neg \varphi \, | \, \varphi.
+\end{align*}\<close>
+
+text \<open>The data type \<open>('a, 'i)hml\<close> formalizes the definition of HML formulas above. It is parameterized by the type of actions \<open>'a\<close> for $\Sigma$
+and an index type \<open>'i\<close>. We use an index sets of arbitrary type \<open>I :: 'i set\<close> and a mapping \<open>F :: 'i \<Rightarrow> ('a, 'i) hml\<close> to formalize
+conjunctions so that each element of \<open>I\<close> is mapped to a formula%
+\footnote{Note that the formalization via an arbitrary set (...) does not yield a valid type, since \<open>set\<close> is not a bounded natural functor.}%.
+\<close>
+
+datatype ('a, 'i)hml =
+TT |
+hml_pos \<open>'a\<close> \<open>('a, 'i)hml\<close> |
+hml_conj "'i set" "'i set" "'i \<Rightarrow> ('a, 'i) hml" 
+
+text \<open>Note that in canonical definitions of HML @{term "TT"} is not usually part of the syntax,
+but is instead synonymous to \<open>\<And>{}\<close>.
+We include @{term "TT"} in the definition to enable Isabelle to infer that the type @{term "hml"} is not empty..
+This formalization allows for conjunctions of arbitrary - even of infinite - width and has been
+taken from \cite{Pohlmann2021ReducingReactive} (Appendix B).\<close>
+
+context lts begin
+
+primrec hml_semantics :: \<open>'s \<Rightarrow> ('a, 's)hml \<Rightarrow> bool\<close>
+(\<open>_ \<Turnstile> _\<close> [50, 50] 50)
+where
+hml_sem_tt: \<open>(_ \<Turnstile> TT) = True\<close> |
+hml_sem_pos: \<open>(p \<Turnstile> (hml_pos \<alpha> \<phi>)) = (\<exists> q. (p \<mapsto>\<alpha> q) \<and> q \<Turnstile> \<phi>)\<close> |
+hml_sem_conj: \<open>(p \<Turnstile> (hml_conj I J \<psi>s)) = ((\<forall>i \<in> I. p \<Turnstile> (\<psi>s i)) \<and> (\<forall>j \<in> J. \<not>(p \<Turnstile> (\<psi>s j))))\<close>
+
+definition HML_true where
+"HML_true \<phi> \<equiv> \<forall>s. s \<Turnstile> \<phi>"
+
+lemma 
+  fixes s::'s
+  assumes "HML_true (hml_conj I J \<Phi>)"
+  shows "\<forall>\<phi> \<in> \<Phi> ` I. HML_true \<phi>"
+  using HML_true_def assms by auto
+
+text \<open>Two states are HML equivalent if they satisfy the same formula.\<close>
+definition HML_equivalent :: \<open>'s \<Rightarrow> 's \<Rightarrow> bool\<close> where
+  \<open>HML_equivalent p q \<equiv> (\<forall> \<phi>::('a, 's) hml. (p \<Turnstile> \<phi>) \<longleftrightarrow> (q \<Turnstile> \<phi>))\<close>
+
+text \<open> An HML formula \<open>\<phi>l\<close> implies another (\<open>\<phi>r\<close>) if the fact that some process \<open>p\<close> satisfies \<open>\<phi>l\<close>
+implies that \<open>p\<close> must also satisfy \<open>\<phi>r\<close>, no matter the process \<open>p\<close>. \<close>
+
+definition hml_impl :: "('a, 's) hml \<Rightarrow> ('a, 's) hml \<Rightarrow> bool" (infix "\<Rrightarrow>" 60)  where
+  "\<phi>l \<Rrightarrow> \<phi>r \<equiv> (\<forall>p. (p \<Turnstile> \<phi>l) \<longrightarrow> (p \<Turnstile> \<phi>r))"
+
+lemma hml_impl_iffI: "\<phi>l \<Rrightarrow> \<phi>r = (\<forall>p. (p \<Turnstile> \<phi>l) \<longrightarrow> (p \<Turnstile> \<phi>r))"
+  using hml_impl_def by force
+
+subsection \<open> Equivalence \<close>
+
+text \<open>
+A HML formula \<open>\<phi>l\<close> is said to be equivalent to some other HML formula \<open>\<phi>r\<close> (written \<open>\<phi>l \<Lleftarrow>\<Rrightarrow> \<phi>r\<close>)
+iff process \<open>p\<close> satisfies \<open>\<phi>l\<close> iff it also satisfies \<open>\<phi>r\<close>, no matter the process \<open>p\<close>.
+
+We have chosen to define this equivalence by appealing to HML formula implication (c.f. pre-order).
+\<close>
+
+definition hml_formula_eq :: "('a, 's) hml \<Rightarrow> ('a, 's) hml \<Rightarrow> bool" (infix "\<Lleftarrow>\<Rrightarrow>" 60)  where
+  "\<phi>l \<Lleftarrow>\<Rrightarrow> \<phi>r \<equiv> \<phi>l \<Rrightarrow> \<phi>r \<and> \<phi>r \<Rrightarrow> \<phi>l"
+
+text \<open> \<open>\<Lleftarrow>\<Rrightarrow>\<close> is truly an equivalence relation. \<close>
+lemma hml_eq_equiv: "equivp (\<Lleftarrow>\<Rrightarrow>)"
+  by (smt (verit, del_insts) equivpI hml_formula_eq_def hml_impl_def reflpI sympI transpI)
+
+lemma equiv_der:
+  assumes "HML_equivalent p q" "\<exists>p'. p \<mapsto>\<alpha> p'"
+  shows "\<exists>p' q'. (HML_equivalent p' q') \<and> q \<mapsto>\<alpha> q'"
+  using assms hml_semantics.simps
+  unfolding HML_equivalent_def 
+  by metis
+
+
+lemma equiv_trans: "transp HML_equivalent"
+  by (simp add: HML_equivalent_def transp_def)
+
+text \<open>
+  A formula distinguishes one state from another if its true for the
+  first and false for the second.
+\<close>
+abbreviation distinguishes ::  \<open>('a, 's) hml \<Rightarrow> 's \<Rightarrow> 's \<Rightarrow> bool\<close> where
+   \<open>distinguishes \<phi> p q \<equiv> p \<Turnstile> \<phi> \<and> \<not> q \<Turnstile> \<phi>\<close>
+
+lemma hml_equiv_sym:
+  shows \<open>symp HML_equivalent\<close>
+unfolding HML_equivalent_def symp_def by simp
+
+text \<open>
+  If two states are not HML equivalent then there must be a
+  distinguishing formula.\<close>
+
+(*assumes that lts is not empty, kann evtl auch aus \<not> HML_equivalent p q gezeigt werden*)
+lemma hml_distinctions:
+  fixes state::"'s"
+  assumes \<open>\<not> HML_equivalent p q\<close>
+  shows \<open>\<exists>\<phi>. distinguishes \<phi> p q\<close>
+proof-
+  from assms have "\<not> (\<forall> \<phi>::('a, 's) hml. (p \<Turnstile> \<phi>) \<longleftrightarrow> (q \<Turnstile> \<phi>))" 
+    unfolding HML_equivalent_def by blast
+  then obtain \<phi>::"('a, 's) hml" where "(p \<Turnstile> \<phi>) \<noteq> (q \<Turnstile> \<phi>)" by blast
+  then have "((p \<Turnstile> \<phi>) \<and> \<not>(q \<Turnstile> \<phi>)) \<or> (\<not>(p \<Turnstile> \<phi>) \<and> (q \<Turnstile> \<phi>))"
+    by blast
+  then show ?thesis
+  proof
+    show "distinguishes \<phi> p q \<Longrightarrow> \<exists>\<phi>. distinguishes \<phi> p q" by blast
+  next
+    assume assm: "\<not> p \<Turnstile> \<phi> \<and> q \<Turnstile> \<phi>"
+    define n\<phi> where "n\<phi> \<equiv>(hml_conj ({}::'s set) 
+                          {state} 
+                          (\<lambda>j. if j = state then \<phi> else undefined))"
+    have "p \<Turnstile> n\<phi> \<and> \<not> q \<Turnstile> n\<phi>" 
+      unfolding n\<phi>_def
+      using hml_semantics.simps assm
+      by force
+    then show ?thesis
+      by blast
+  qed
+qed
+
+end (* context lts *)
+end
