Transition_Systems.thy
@@ -8,65 +8,78 @@ begin
 section \<open>Labeled Transition Systems\<close>
 text \<open>\label{sec:LTS}\<close>
 
-text \<open>- modelling (reactive) systems\\
-- model for parallel computation (Kel)\\
-- formalization of deadlock (Kel)\\
-- models "parallelism" - for q there may be many states q' such that q -> q' -> model non determinism\\\<close>
-
-text \<open>Harel:\\
-- reactive systems: continuously respond to external inputs\\
-- doens't perform function but maintains relationship with its environment\<close>
-
-text \<open>Labeled Transition Systems (LTS) serve as models for representing the behavior of systems (Kel76). 
-An LTS consists of three components: processes, actions, and transitions. Processes represent momentary states or configurations of a system. Actions denote the events or operations that can occur within the system.
+text \<open>As mentioned in (Introduction), labeled transition systems are formal models used to describe the behavior of reactive systems.
+A LTS consists of three components: processes, actions, and transitions. Processes represent momentary states or configurations of a system. Actions denote the events or operations that can occur within the system.
 The outgoing transitions of each process correspond to the actions the system can perform in that state, yielding a subsequent state.
-\<close>
+A process may have multiple outgoing transitions labeled with the same or different actions. This signifies that the system can choose any of these transitions nondeterministically
+\footnote{Note that "nondeterministic" has been used  differently in some of the literature (citation needed). In the context of reactive systems, 
+all transitions are directly triggered by external actions or events and represent synchronization with the environment.
+The next state of the system is then uniquely determined by its current state and the external action. In that sense the behavior of the system is deterministic.}.
+The semantic equivalences treated in (Glabbeeck) are defined entirely in terms of action relations.
+We treat processes as being \textit{sequential}, meaning it can perform at most one action at a time, and instantanious.
+Note that many modeling methods of systems use a special $\tau$-action to represent internal behavior. However, in our definition of LTS, 
+internal behavior is not considered.\<close>
 
-subsubsection \<open>Definition 1 (Labeled transition Systems)\<close>
+subsubsection \<open>Definition 1.1 (Labeled transition Systems)\<close>
 
-text \<open>A Labelled Transition System (LTS) is a tuple $\mathcal{S} = (\Proc, \Act, \rightarrow)$ where $\Proc$ is the set of processes, 
-$\Act$ is the set of actions and $\rightarrow$ $\subseteq \Proc \times \Act \times \Proc$ is a transition relation.\\
+text \<open>A \textit{Labeled Transition System} (LTS) is a tuple $\mathcal{S} = (\Proc, \Act, \rightarrow)$ where $\Proc$ is the set of processes, 
+$\Act$ is the set of actions and $\rightarrow$ $\subseteq \Proc \times \Act \times \Proc$ is a transition relation.
+We write $p \rightarrow{\alpha} p'$ for $(p, \alpha, p')\in \rightarrow$.\<close>
 
-In concurrency theory, it is customary that the semantics of Reactive Systems are given in terms of labelled transition systems.
-The processes represent the states a reactive system can be in. A transition of one state into another, 
-caused by performing an action, can be understood as moving along the corresponding edge in the transition relation. \\
+text \<open>Actions and processes are formalized using type variable \<open>'a\<close> and \<open>'s\<close>, respectively. As only actions and states involved in the transition relation are relevant, 
+the set of transitions uniquely defines a specific LTS. We express this relationship using the predicate \<open>tran\<close>. We associate it with a more readable notation (\<open>p \<mapsto>\<alpha> p'\<close> for $p \xrightarrow{\alpha} p'$).\<close>
 
-- Example?\\
-
-- examples (to reuse later?)???
-\<close>
-
-subsubsection \<open>Some more Definitions\<close>
-
-text \<open>The $\alpha$-derivatives of a process are the processes that can be reached with one $\alpha$-transition:\<close>
-
-
-text \<open>
-- image finite? nötig?\\
-- image countable?
-- initial actions
-- deadlock
-- relevant actions?
-- step sequence!
-- \<close>
-
-subsection \<open>Isabelle\<close>
-
-text \<open>Zustände: \<open>'s\<close> und Aktionen \<open>'a\<close>, Transitionsrelation ist locale trans. Ein LTS wird dann durch
-seine Transitionsrelation definiert.\<close>
 locale lts = 
   fixes tran :: \<open>'s \<Rightarrow> 'a \<Rightarrow> 's \<Rightarrow> bool\<close> 
     ("_ \<mapsto>_ _" [70, 70, 70] 80)
 begin
 
+text \<open>Example... (to reuse later?)\<close>
+
+text \<open>We introduce some concepts to better talk about LTS. Note that these Isabelle definitions are only defined in the \<open>context\<close> of LTS.\<close>
+
+subsubsection \<open>Definition 1.2\<close>
+
+text \<open>The \textit{$\alpha$-derivatives} of a state refer to the set of states that can be reached with an $\alpha$-transition:
+$$mathit{Der} (p, \alpha) = \{ p' \mid p \xrightarrow{\alpha} p' \}.$$\<close>
+
 abbreviation derivatives :: \<open>'s \<Rightarrow> 'a \<Rightarrow> 's set\<close>
   where
 \<open>derivatives p \<alpha> \<equiv> {p'. p \<mapsto>\<alpha> p'}\<close>
 
-text \<open>Transition System is image-finite\<close>
+text \<open>The set of \textit{initial actions} of a process $p$ is defined by: 
+$$I(p)={\alpha \in Act \mid \exists p'. p \xrightarrow{\alpha} p'}$$\<close>
+
+abbreviation initial_actions:: \<open>'s \<Rightarrow> 'a set\<close>
+  where
+\<open>initial_actions p \<equiv> {\<alpha>|\<alpha>. (\<exists>p'. p \<mapsto>\<alpha> p')}\<close>
+
+text \<open>The step sequence relation $\xrightarrow{\sigma}*$ for $\sigma \in \Act$ is the reflexive transitive closure of $p \xrightarrow{\alpha} p'$.
+It is defined recursively by:
+\begin{align*}
+  p &\xrightarrow{\varepsilon}^* p \\
+  p &\xrightarrow{\alpha} p' \text{ with } \alpha \in \text{Act} \text{ and } p' \xrightarrow{\sigma}^* p'' \text{ implies } p' \xrightarrow{\sigma}^* p''
+\end{align*}
+\<close>
+
+inductive step_sequence :: \<open>'s \<Rightarrow> 'a list \<Rightarrow> 's \<Rightarrow> bool\<close> (\<open>_ \<mapsto>$ _ _\<close>[70,70,70] 80) where
+\<open>p \<mapsto>$ [] p\<close> |
+\<open>p \<mapsto>$ (a#rt) p''\<close> if \<open>\<exists>p'. p \<mapsto> a p' \<and> p' \<mapsto>$ rt p''\<close>
+
+text \<open>$p$ is image-finite if for each $\alpha \in \Act$ the set $mathit{Der} (p, \alpha)$ is finite.
+An LTS is image-finite if each $p \in \Proc$ is image-finite:
+"$$\forall p \in\Proc, \alpha \in \Act. mathit{Der} (p, \alpha)$$ is finite.\<close>
 
 definition image_finite where
 \<open>image_finite \<equiv> (\<forall>p \<alpha>. finite (derivatives p \<alpha>))\<close>
+
+text \<open>We say that a process is in a \textit{deadlock} if no observation is possible. That is:
+$$\mathit{deadlock} p = (\forall\alpha .\mathit{deadlock} p \alpha = \varnothing)$$\<close>
+
+abbreviation deadlock :: \<open>'s \<Rightarrow> bool\<close> where
+\<open>deadlock p \<equiv> (\<forall>\<alpha>. derivatives p \<alpha> = {})\<close>
+
+text \<open>nötig?\<close>
 
 definition image_countable :: \<open>bool\<close>
   where \<open>image_countable \<equiv> (\<forall> p \<alpha>. countable (derivatives p \<alpha>))\<close>
@@ -75,21 +88,10 @@ text \<open>stimmt definition? definition benötigt nach umstieg auf sets?\<clos
 definition lts_finite where
 \<open>lts_finite \<equiv> (finite (UNIV :: 's set))\<close>
 
-abbreviation initial_actions:: \<open>'s \<Rightarrow> 'a set\<close>
-  where
-\<open>initial_actions p \<equiv> {\<alpha>|\<alpha>. (\<exists>p'. p \<mapsto>\<alpha> p')}\<close>
-
-abbreviation deadlock :: \<open>'s \<Rightarrow> bool\<close> where
-\<open>deadlock p \<equiv> (\<forall>a. derivatives p a = {})\<close>
-
-text \<open>nötig?\<close>
 abbreviation relevant_actions :: \<open>'a set\<close>
   where
 \<open>relevant_actions \<equiv> {a. \<exists>p p'. p \<mapsto>a p'}\<close>
 
-inductive step_sequence :: \<open>'s \<Rightarrow> 'a list \<Rightarrow> 's \<Rightarrow> bool\<close> (\<open>_ \<mapsto>$ _ _\<close>[70,70,70] 80) where
-\<open>p \<mapsto>$ [] p\<close> |
-\<open>p \<mapsto>$ (a#rt) p''\<close> if \<open>\<exists>p'. p \<mapsto> a p' \<and> p' \<mapsto>$ rt p''\<close>
 
 end
 
